almost there, but Qed fails?

theories/Example_1_1.v
@@ -1,7 +1,11 @@
 
 From LogRel.AutoSubst Require Import core unscoped Ast Extra.
-From LogRel Require Import Utils BasicAst Context DeclarativeTyping.
+From LogRel Require Import Utils Notations BasicAst Context GenericTyping DeclarativeTyping DeclarativeInstance BundledAlgorithmicTyping.
+From PartialFun Require Import Monad PartialFun.
 From LogRel.Decidability Require Import Functions Soundness Completeness Termination.
+
+Import DeclarativeTypingProperties.
+Import IndexedDefinitions.
 
 #[local] Definition infer (Γ : context) (t : term) : Fueled (result term) :=
   (fueled typing 1000 (inf_state;Γ;tt;t)).
@@ -21,6 +25,9 @@ Definition rec2pi1 (p: term) : term := tFst p.
 Definition rec2pi2 (p: term) : term := tSnd p.
 Eval vm_compute in (infer ε (mkRec2 tNat tNat tZero tZero)).
 
+Definition rec2N := rec2 tNat tNat.
+Definition mkRec2N (a b : term) := mkRec2 tNat tNat a b.
+
 Definition rec3 (A B C: term) : term := tSig A (rec2 B C)⟨↑⟩.
 Definition mkRec3 (A B C: term) (a b c: term) : term := tPair A (rec2 B C)⟨↑⟩ a (mkRec2 B C b c).
 Definition rec3pi1 (p: term) : term := tFst p.
@@ -28,6 +35,11 @@ Definition rec3pi2 (p: term) : term := tFst (tSnd p).
 Definition rec3pi3 (p: term) : term := tSnd (tSnd p).
 Eval vm_compute in (infer ε (mkRec3 tNat tNat tNat tZero tZero tZero)).
 
+Definition rec3N := rec3 tNat tNat tNat.
+Definition mkRec3N (a b c : term) := mkRec3 tNat tNat tNat a b c.
+
+Definition idtype A := (arr A A).
+Definition idty_rec2N := idtype rec2N.
 
 Fixpoint nat_to_tNat (n: nat) :=
   match n with
@@ -37,37 +49,71 @@ Fixpoint nat_to_tNat (n: nat) :=
 Definition forty_two : term := nat_to_tNat 42.
 
 Definition glue : term :=
-  tLambda (rec2 tNat tNat)
-    (mkRec3 tNat tNat tNat
+  tLambda rec2N
+    (mkRec3N
        (rec2pi1 (tRel 0))
        (rec2pi2 (tRel 0))
        forty_two
     ).
 Eval vm_compute in (infer ε glue).
+Check (eq_refl : infer ε glue = Success (ok (arr rec2N rec3N))).
 
 Definition glue_retr : term :=
-  tLambda (rec3 tNat tNat tNat)
-    (mkRec2 tNat tNat
+  tLambda rec3N
+    (mkRec2N
        (rec3pi1 (tRel 0))
        (rec3pi2 (tRel 0))
     ).
 Eval vm_compute in (infer ε glue_retr).
+Check (eq_refl : infer ε glue_retr = Success (ok (arr rec3N rec2N))).
 
-Definition idtest : term :=
-  tLambda (rec2 tNat tNat)
-    (mkRec2 tNat tNat
-       (rec2pi1 (tRel 0))
-       (rec2pi2 (tRel 0))
-    ).
-Eval vm_compute in (infer ε idtest).
-Eval vm_compute in (infer ε (idterm (rec2 tNat tNat))).
+Eval vm_compute in (conv_tm ε idty_rec2N (idterm rec2N) (comp rec2N glue_retr glue)).
 
+Definition map_example :=
+  tLambda (tList rec2N) (tMap rec3N rec2N glue_retr (tMap rec2N rec3N glue (tRel 0))).
 
-Eval vm_compute in (conv_tm ε (rec2 tNat tNat) idtest (idterm (rec2 tNat tNat))).
+Eval vm_compute in (conv_tm ε (idtype (tList rec2N)) map_example (idterm (tList rec2N))).
 
+Lemma map_example_conv : conv_tm ε (idtype (tList rec2N)) map_example (idterm (tList rec2N)) = Success (ok tt).
+Proof.
+  reflexivity.
+Qed.
 
+Lemma map_example_ty_eq : infer ε map_example = Success (ok (idtype (tList rec2N))).
+Proof.
+  reflexivity.
+Qed.
 
+Lemma map_example_ty : [ε |- map_example : idtype (tList rec2N)].
+Proof.
+  pose proof map_example_ty_eq as e.
+  unfold infer in e.
+  eapply (fueled_graph_sound typing _ (inf_state; _)) in e.
+  apply implem_typing_sound, algo_typing_sound in e.
+  + assumption.
+  + constructor.
+Fail Qed. (* Stack overflow *)
+Admitted.
 
+Lemma idterm_ty : infer ε (idterm (tList rec2N)) = Success (ok (idtype (tList rec2N))).
+Proof.
+  reflexivity.
+Qed.
 
-
-
+Theorem example_1_1_conv : [ε |- map_example ≅ idterm (tList rec2N) : idtype (tList rec2N)].
+Proof.
+  pose proof map_example_conv as e.
+  unfold conv_tm in e.
+  eapply (fueled_graph_sound conv) in e.
+  apply implem_conv_sound, algo_conv_sound in e.
+  - assumption.
+  - apply map_example_ty.
+  - clear.
+    pose proof idterm_ty as e.
+    unfold infer in e.
+    eapply (fueled_graph_sound typing _ (inf_state; _)) in e.
+    apply implem_typing_sound, algo_typing_sound in e.
+    + assumption.
+    + constructor.
+Fail Qed.
+Admitted.
